Tests/DTLC/Sanity.lean
@@ -133,40 +133,41 @@ attribute [local simp] Trm.get1st Trm.get2nd Trm.get1stOnTuple Trm.get2ndOnTuple
 attribute [local simp] Trm.apply1stOn2ndFn Trm.apply1stOn2ndFnOnTuple
 attribute [local simp] Trm.applyidFnOnItself Trm.idFnOnFalse2
 
-example : ((Trm.false : Trm I).eval 0) = none := rfl
-example : ((Trm.false : Trm I).eval 1) = some ((Val.primitive "false") : Val I) := rfl
-example : ((Trm.false : Trm I).eval 2) = some ((Val.primitive "false") : Val I) := rfl
-example : ((Trm.idFnOnFalse : Trm I).eval 0) = none := rfl
+example : ((Trm.false : Trm I).eval 0) = .outOfFuel := rfl
+example : ((Trm.false : Trm I).eval 1) = .some ((Val.primitive "false") : Val I) := rfl
+example : ((Trm.false : Trm I).eval 2) = .some ((Val.primitive "false") : Val I) := rfl
+example : ((Trm.idFnOnFalse : Trm I).eval 0) = .outOfFuel := rfl
 
 example : ((Trm.idFnOnFalse : Trm I).eval 2) =
-    some ((Val.primitive "false") : Val I) := by
+    .some ((Val.primitive "false") : Val I) := by
   simp
 
-example : ((Trm.get1stOnTuple : Trm I).eval 1) = none := rfl
+example : ((Trm.get1stOnTuple : Trm I).eval 1) = .error := rfl
 
 example : ((Trm.get1stOnTuple : Trm I).eval 3) =
-    some ((Val.primitive "false") : Val I) := by
+    .some ((Val.primitive "false") : Val I) := by
   simp
 
 example : ((Trm.get2ndOnTuple : Trm I).eval 3) =
-    some ((Val.primitive "true") : Val I) := by
+    .some ((Val.primitive "true") : Val I) := by
   simp
 
-example : ((Trm.apply1stOn2ndFnOnTuple : Trm I).eval 2) = none := rfl
+example : ((Trm.apply1stOn2ndFnOnTuple : Trm I).eval 2) = .error := rfl
 
 example : ((Trm.apply1stOn2ndFnOnTuple : Trm I).eval 4) =
-    some ((Val.primitive "false") : Val I) := by
+    .some ((Val.primitive "false") : Val I) := by
   simp
 
-example : (((Trm.applyidFnOnItself : Trm I).eval 0).isNone) = true := rfl
+example : ((Trm.applyidFnOnItself : Trm I).eval 0) = .outOfFuel := rfl
 
-example : (((Trm.applyidFnOnItself : Trm I).eval 2).isSome) = true := by
-  simp
+example : ((Trm.applyidFnOnItself : Trm I).eval 2) =
+    .some ((Val.idFn : Val I)) := by
+  simp [Val.idFn]
 
-example : ((Trm.idFnOnFalse2 : Trm I).eval 1) = none := rfl
+example : ((Trm.idFnOnFalse2 : Trm I).eval 1) = .error := rfl
 
 example : ((Trm.idFnOnFalse2 : Trm I).eval 3) =
-    some ((Val.primitive "false") : Val I) := by
+    .some ((Val.primitive "false") : Val I) := by
   simp
 
 end Eval
